src/ldrfra/LocalDRFRA.v
@@ -1,0 +1,53 @@
+Require Import Lia.
+Require Import Bool.
+Require Import RelationClasses.
+Require Import Program.
+
+From sflib Require Import sflib.
+From Paco Require Import paco.
+
+From PromisingLib Require Import Axioms.
+From PromisingLib Require Import Basic.
+From PromisingLib Require Import DataStructure.
+From PromisingLib Require Import DenseOrder.
+From PromisingLib Require Import Loc.
+From PromisingLib Require Import Language.
+From PromisingLib Require Import Event.
+
+Require Import Time.
+Require Import View.
+Require Import BoolMap.
+Require Import Promises.
+Require Import Cell.
+Require Import Memory.
+Require Import TView.
+Require Import Global.
+Require Import Local.
+Require Import Thread.
+Require Import Configuration.
+Require Import PFConfiguration.
+Require Import Behavior.
+
+Require Import OrdStep.
+Require Import Stable.
+Require Import WStep.
+Require Import PFtoRA.
+Require Import RARace.
+
+Set Implicit Arguments.
+
+
+(* LDRF-RA theorem *)
+
+Theorem local_drf_ra L
+        s
+        (RACEFREE: RARace.racefree_syn L s):
+  behaviors (PFConfiguration.step ThreadEvent.get_machine_event_pf) (Configuration.init s) <2=
+  behaviors (@OrdConfiguration.step L Ordering.acqrel Ordering.acqrel) (Configuration.init s).
+Proof.
+  hexploit RARace.racefree_implies; eauto. i.
+  specialize (PFtoRA.init_sim_conf L s). intro SIM.
+  specialize (PFtoRA.init_wf_pf s). intro WF_PF.
+  specialize (PFtoRA.init_wf_ra L s). intro WF_RA.
+  ii. eapply PFtoRA.sim_conf_behavior; eauto.
+Qed.
