src/ldrfra/PFtoRA.v
@@ -1,0 +1,365 @@
+Require Import Lia.
+Require Import Bool.
+Require Import RelationClasses.
+
+From sflib Require Import sflib.
+From Paco Require Import paco.
+
+From PromisingLib Require Import Axioms.
+From PromisingLib Require Import Basic.
+From PromisingLib Require Import DataStructure.
+From PromisingLib Require Import DenseOrder.
+From PromisingLib Require Import Loc.
+From PromisingLib Require Import Language.
+From PromisingLib Require Import Event.
+
+Require Import Time.
+Require Import View.
+Require Import BoolMap.
+Require Import Promises.
+Require Import Cell.
+Require Import Memory.
+Require Import TView.
+Require Import Global.
+Require Import Local.
+Require Import Thread.
+Require Import Configuration.
+Require Import PFConfiguration.
+Require Import Behavior.
+
+Require Import OrdStep.
+Require Import Writes.
+Require Import WStep.
+Require Import Stable.
+Require Import PFtoRASim.
+Require Import PFtoRAThread.
+
+Set Implicit Arguments.
+
+
+Module PFtoRA.
+  Section PFtoRA.
+    Variable L: Loc.t -> bool.
+
+    (* well-formedness *)
+
+    Variant wf_pf (c: Configuration.t): Prop :=
+    | wf_pf_intro
+        (WF: Configuration.wf c)
+        (PRM: forall tid lang st lc
+                (TH: IdentMap.find tid (Configuration.threads c) = Some (existT _ lang st, lc)),
+            Local.promises lc = BoolMap.bot)
+        (GPRM: Global.promises (Configuration.global c) = BoolMap.bot)
+    .
+
+    Variant wf_ra (rels: Writes.t) (c: Configuration.t): Prop :=
+    | wf_ra_intro
+        (WF: Configuration.wf c)
+        (RELS: Writes.wf L rels (Global.memory (Configuration.global c)))
+        (PRM: forall tid lang st lc
+                (TH: IdentMap.find tid (Configuration.threads c) = Some (existT _ lang st, lc)),
+            Local.promises lc = BoolMap.bot)
+        (GPRM: Global.promises (Configuration.global c) = BoolMap.bot)
+    .
+
+    Lemma wf_pf_thread
+          c tid lang st lc
+          (WF: wf_pf c)
+          (FIND: IdentMap.find tid (Configuration.threads c) = Some (existT _ lang st, lc)):
+      PFtoRAThread.wf_pf (Thread.mk _ st lc (Configuration.global c)).
+    Proof.
+      inv WF. inv WF0. inv WF.
+      econs; eauto.
+    Qed.
+
+    Lemma wf_ra_thread
+          rels c tid lang st lc
+          (WF: wf_ra rels c)
+          (FIND: IdentMap.find tid (Configuration.threads c) = Some (existT _ lang st, lc)):
+      PFtoRAThread.wf_ra L rels (Thread.mk _ st lc (Configuration.global c)).
+    Proof.
+      inv WF. inv WF0. inv WF.
+      econs; eauto.
+    Qed.
+
+    Lemma step_pf_future
+          e tid c1 c2
+          (WF1: wf_pf c1)
+          (STEP: PFConfiguration.estep e tid c1 c2):
+      <<WF2: wf_pf c2>>.
+    Proof.
+      exploit PFConfiguration.estep_future; try apply WF1; eauto. i. des.
+      inv STEP. ss.
+      exploit wf_pf_thread; eauto. i.
+      exploit PFtoRAThread.step_pf_future; eauto. i. des. inv x1. ss.
+      econs; ss. i. Configuration.simplify.
+      inv WF1. eauto.
+    Qed.
+
+    Lemma step_ra_future
+          ordr ordw
+          e tid rels1 rels2 c1 c2
+          (WF1: wf_ra rels1 c1)
+          (ORD: Ordering.le Ordering.plain ordw)
+          (STEP: WConfiguration.step L ordr ordw e tid rels1 rels2 c1 c2):
+      <<WF2: wf_ra rels2 c2>>.
+    Proof.
+      exploit WConfiguration.step_future; try eapply WF1; eauto. i. des.
+      inv STEP. ss.
+      exploit wf_ra_thread; eauto. i.
+      hexploit WThread.step_writes_wf; eauto; try apply x0. s. i.
+      exploit PFtoRAThread.step_ra_future; eauto. i. des. inv x1. ss.
+      econs; ss. i. Configuration.simplify; ss.
+      inv WF1. eauto.
+    Qed.
+
+    Lemma steps_pf_future
+          c1 c2
+          (WF1: wf_pf c1)
+          (STEPS: rtc (PFConfiguration.all_step) c1 c2):
+      <<WF2: wf_pf c2>>.
+    Proof.
+      induction STEPS; ss. inv H.
+      exploit step_pf_future; eauto.
+    Qed.
+
+    Lemma steps_ra_future
+          ordr ordw
+          rels1 rels2 c1 c2
+          (WF1: wf_ra rels1 c1)
+          (ORD: Ordering.le Ordering.plain ordw)
+          (STEPS: WConfiguration.steps L ordr ordw rels1 rels2 c1 c2):
+      <<WF2: wf_ra rels2 c2>>.
+    Proof.
+      induction STEPS; ss.
+      exploit step_ra_future; eauto.
+    Qed.
+
+
+    (* sim *)
+
+    Variant sim_thread_sl (rels: Writes.t) (gl_pf gl_ra: Global.t):
+      forall (sl_pf sl_ra: {lang: language & Language.state lang} * Local.t), Prop :=
+    | sim_thread_sl_intro
+        lang st_pf lc_pf st_ra lc_ra
+        (SIM: PFtoRAThread.sim_thread L rels
+                                      (Thread.mk lang st_pf lc_pf gl_pf)
+                                      (Thread.mk lang st_ra lc_ra gl_ra)):
+        sim_thread_sl rels gl_pf gl_ra
+                      (existT _ lang st_pf, lc_pf) (existT _ lang st_ra, lc_ra)
+    .
+
+    Variant sim_conf (rels: Writes.t): forall (c_pf c_ra: Configuration.t), Prop :=
+    | sim_conf_intro
+        ths_pf gl_pf
+        ths_ra gl_ra
+        (THS: forall tid,
+            option_rel
+              (sim_thread_sl rels gl_pf gl_ra)
+              (IdentMap.find tid ths_pf)
+              (IdentMap.find tid ths_ra)):
+        sim_conf rels
+                 (Configuration.mk ths_pf gl_pf)
+                 (Configuration.mk ths_ra gl_ra)
+    .
+
+    Lemma init_wf_pf syn:
+      wf_pf (Configuration.init syn).
+    Proof.
+      econs; eauto using Configuration.init_wf.
+      i. ss.
+      unfold Threads.init in *.
+      rewrite IdentMap.Facts.map_o in *.
+      destruct (@UsualFMapPositive.UsualPositiveMap'.find
+                  (@sigT _ (@Language.syntax ProgramEvent.t)) tid syn); inv TH.
+      apply inj_pair2 in H1. subst. ss.
+    Qed.
+
+    Lemma init_wf_ra syn:
+      wf_ra [] (Configuration.init syn).
+    Proof.
+      econs; eauto using Configuration.init_wf; i; ss.
+      - econs; i; ss.
+        unfold Memory.get, Memory.init, Cell.get, Cell.init in *. ss.
+        apply DOMap.singleton_find_inv in GET. des. inv GET0. ss.
+      -unfold Threads.init in *.
+        rewrite IdentMap.Facts.map_o in *.
+        destruct (@UsualFMapPositive.UsualPositiveMap'.find
+                    (@sigT _ (@Language.syntax ProgramEvent.t)) tid syn); inv TH.
+        apply inj_pair2 in H1. subst. ss.
+    Qed.
+
+    Lemma init_sim_conf syn:
+      sim_conf [] (Configuration.init syn) (Configuration.init syn).
+    Proof.
+      econs; ss. i. unfold option_rel.
+      destruct (IdentMap.find tid (Threads.init syn)) as [[[lang st] lc]|] eqn:FIND; ss.
+      unfold Threads.init in *.
+      rewrite IdentMap.Facts.map_o in *.
+      destruct (@UsualFMapPositive.UsualPositiveMap'.find
+                  (@sigT _ (@Language.syntax ProgramEvent.t)) tid syn); inv FIND.
+      apply inj_pair2 in H1. subst.
+      econs. econs; ss.
+      (* - econs; ss; try refl. econs; try refl. ii. *)
+      (*   rewrite Memory.bot_get. ss. *)
+      (* - econs; ss. econs; ss; eauto. i. *)
+      (*   unfold Memory.get, Memory.init, Cell.get, Cell.init in *. ss. *)
+      (*   apply DOMap.singleton_find_inv in GET. des. inv GET0. ss. *)
+      - econs; ss.
+        + econs; ss. econs; ss. i. condtac; ss. refl.
+        + econs; ss; i.
+          * unfold Memory.get, Memory.init, Cell.get, Cell.init in *. ss.
+            apply DOMap.singleton_find_inv in GET_SRC. des. inv GET_SRC0.
+            esplits; ss. econs; ss. condtac; ss.
+          * unfold Memory.get, Memory.init, Cell.get, Cell.init in *. ss.
+            apply DOMap.singleton_find_inv in GET_TGT. des. inv GET_TGT0.
+            esplits; ss. econs; ss. condtac; ss.
+          * unfold Memory.get, Memory.init, Cell.get, Cell.init in *. ss.
+            apply DOMap.singleton_find_inv in GET_TGT. des. inv GET_TGT0. ss.
+      - econs; ss. ii.
+        unfold Memory.get, Memory.init, Cell.get, Cell.init in *. ss.
+        apply DOMap.singleton_find_inv in GET. des. inv GET0.
+      - econs; ss. ii.
+        unfold Memory.get, Memory.init, Cell.get, Cell.init in *. ss.
+        apply DOMap.singleton_find_inv in GET. des. inv GET0.
+      - econs; ss. ii. des; ss.
+        unfold Memory.get, Memory.init, Cell.get, Cell.init in *. ss.
+        apply DOMap.singleton_find_inv in GET. des. inv GET1.
+    Qed.
+
+    Lemma sim_conf_terminal
+          rels c_pf c_ra
+          (WF_RA: wf_ra rels c_ra)
+          (SIM: sim_conf rels c_pf c_ra)
+          (TERMINAL: Configuration.is_terminal c_pf):
+      Configuration.is_terminal c_ra.
+    Proof.
+      ii. inv SIM. specialize (THS tid).
+      unfold option_rel in *. ss. des_ifs.
+      destruct p as [[]]. inv THS.
+      Configuration.simplify.
+      inv SIM. inv SIM_RA. ss. subst.
+      exploit TERMINAL; eauto. i. des.
+      split; ss.
+      inv WF_RA. eauto.
+    Qed.
+
+
+    (* step *)
+
+    Lemma sim_conf_step
+          rels1 c1_pf c1_ra
+          tid e_pf c2_pf
+          (SIM1: sim_conf rels1 c1_pf c1_ra)
+          (WF1_PF: wf_pf c1_pf)
+          (WF1_RA: wf_ra rels1 c1_ra)
+          (STEP: PFConfiguration.estep e_pf tid c1_pf c2_pf):
+      (exists e_ra rels2 c2_ra,
+          (<<STEP_RA: WConfiguration.step L Ordering.acqrel Ordering.acqrel
+                                          e_ra tid rels1 rels2 c1_ra c2_ra>>) /\
+          (<<EVENT_RA: PFtoRASim.sim_event e_ra e_pf>>) /\
+          (<<SIM2: sim_conf rels2 c2_pf c2_ra>>)) \/
+      (<<RACE: RARaceW.ra_race_steps L Ordering.acqrel Ordering.acqrel rels1 c1_ra>>).
+    Proof.
+      dup SIM1. inv SIM0. inv STEP. ss.
+      dup THS. specialize (THS0 tid). unfold option_rel in THS0. des_ifs.
+      inv THS0. apply inj_pair2 in H1. subst.
+      exploit wf_pf_thread; eauto. s. i.
+      exploit wf_ra_thread; try exact WF1_RA; eauto. s. i.
+      exploit PFtoRAThread.sim_thread_step; eauto. i. des; cycle 1.
+      { right. unfold RARaceW.ra_race_steps.
+        esplits; [econs 1|..]; eauto.
+      }
+      destruct e2_ra as [st2_ra lc2_ra gl2_ra].
+      left. esplits.
+      - econs; eauto.
+      - ss.
+      - econs; ss. i.
+        repeat rewrite IdentMap.gsspec. condtac; ss.
+        specialize (THS tid0). unfold option_rel in THS. des_ifs. inv THS. ss.
+        inv SIM0. econs. econs; s.
+        + inv SIM_RA. ss. subst.
+          inv SIM2. inv SIM_RA. ss.
+        + econs; try apply SIM2; try apply NORMAL_PF.
+        + econs; try apply SIM2; try apply NORMAL_RA.
+        + econs; s; try apply SIM2; try apply STABLE_RA.
+          exploit WThread.step_future; try exact STEP_RA; try apply x1. s. i. des.
+          exploit wf_ra_thread; try exact WF1_RA; try eapply Heq2. s. i.
+          exploit Stable.future_stable_tview;
+            try eapply STABLE_RA; try apply x2; try apply GL_FUTURE; eauto.
+    Qed.
+
+    Lemma sim_conf_steps
+          rels1 c1_pf c1_ra
+          c2_pf
+          (SIM1: sim_conf rels1 c1_pf c1_ra)
+          (WF1_PF: wf_pf c1_pf)
+          (WF1_RA: wf_ra rels1 c1_ra)
+          (STEPS: rtc PFConfiguration.all_step c1_pf c2_pf):
+      (exists rels2 c2_ra,
+          (<<STEPS_RA: WConfiguration.steps L Ordering.acqrel Ordering.acqrel rels1 rels2 c1_ra c2_ra>>) /\
+          (<<SIM2: sim_conf rels2 c2_pf c2_ra>>)) \/
+      (<<RACE: RARaceW.ra_race_steps L Ordering.acqrel Ordering.acqrel rels1 c1_ra>>).
+    Proof.
+      revert rels1  c1_ra SIM1 WF1_PF WF1_RA.
+      induction STEPS; i.
+      { left. esplits; try by econs 1. ss. }
+      inv H. exploit sim_conf_step; eauto. i. des; eauto.
+      exploit step_pf_future; eauto. i. des.
+      exploit step_ra_future; try exact STEP_RA; eauto. i. des.
+      exploit IHSTEPS; eauto. i. des.
+      - left. esplits; (try by econs 2; eauto); ss.
+      - right. unfold RARaceW.ra_race_steps in *. des.
+        esplits; [econs 2; eauto|..]; eauto.
+    Qed.
+
+
+    (* behaviors *)
+
+    Lemma sim_conf_behavior
+          rels c_pf c_ra
+          (SIM: sim_conf rels c_pf c_ra)
+          (WF_PF: wf_pf c_pf)
+          (WF_RA: wf_ra rels c_ra)
+          (RACEFREE: RARaceW.racefree L Ordering.acqrel Ordering.acqrel rels c_ra):
+      behaviors (PFConfiguration.step ThreadEvent.get_machine_event_pf) c_pf <2=
+      behaviors (@OrdConfiguration.step L Ordering.acqrel Ordering.acqrel) c_ra.
+    Proof.
+      i. revert rels  c_ra SIM WF_PF WF_RA RACEFREE.
+      induction PR; i.
+      - econs 1. eapply sim_conf_terminal; eauto.
+      - inv STEP. exploit sim_conf_step; eauto. i. des.
+        + exploit WConfiguration.step_ord_step; eauto. i.
+          inv EVENT_RA; ss. inv H0.
+          econs 2.
+          { replace (MachineEvent.syscall e2) with
+              (ThreadEvent.get_machine_event_pf (ThreadEvent.syscall e2)) by ss.
+            econs; eauto.
+          }
+          { hexploit RARaceW.step_racefree; eauto. i.
+            exploit step_pf_future; eauto. i. des.
+            exploit step_ra_future; try exact STEP_RA; eauto.
+          }
+          { ss. }
+        + exfalso. unfold RARaceW.ra_race_steps in *. des. eauto.
+      - inv STEP. exploit sim_conf_step; eauto. i. des.
+        + exploit WConfiguration.step_ord_step; eauto. i.
+          econs 3.
+          replace MachineEvent.failure with (ThreadEvent.get_machine_event_pf e_ra); [econs; eauto|].
+          inv EVENT_RA; ss.
+        + exfalso. unfold RARaceW.ra_race_steps in *. des. eauto.
+      - inv STEP. exploit sim_conf_step; eauto. i. des.
+        + exploit WConfiguration.step_ord_step; eauto. i.
+          econs 4.
+          { replace MachineEvent.silent with (ThreadEvent.get_machine_event_pf e_ra); cycle 1.
+            { inv EVENT_RA; ss. }
+            econs; eauto.
+          }
+          hexploit RARaceW.step_racefree; eauto. i.
+          exploit step_pf_future; eauto. i. des.
+          exploit step_ra_future; try exact STEP_RA; eauto.
+        + exfalso. unfold RARaceW.ra_race_steps in *. des. eauto.
+      - econs 5.
+    Qed.
+  End PFtoRA.
+End PFtoRA.
