src/ldrfra/RARace.v
@@ -1,0 +1,189 @@
+Require Import Lia.
+Require Import Bool.
+Require Import RelationClasses.
+Require Import Program.
+
+From sflib Require Import sflib.
+From Paco Require Import paco.
+
+From PromisingLib Require Import Axioms.
+From PromisingLib Require Import Basic.
+From PromisingLib Require Import DataStructure.
+From PromisingLib Require Import DenseOrder.
+From PromisingLib Require Import Loc.
+From PromisingLib Require Import Language.
+From PromisingLib Require Import Event.
+
+Require Import Time.
+Require Import View.
+Require Import BoolMap.
+Require Import Promises.
+Require Import Cell.
+Require Import Memory.
+Require Import TView.
+Require Import Global.
+Require Import Local.
+Require Import Thread.
+Require Import Configuration.
+Require Import PFConfiguration.
+Require Import Behavior.
+
+Require Import OrdStep.
+Require Import Writes.
+Require Import WStep.
+
+Set Implicit Arguments.
+
+
+Module RARace.
+Section RARACE.
+  Variable L: Loc.t -> bool.
+
+  Definition wr_race (loc: Loc.t) (to: Time.t) (ordw: Ordering.t) (tview: TView.t) (ord: Ordering.t): Prop :=
+    (<<LOC: L loc>>) /\
+    (<<HIGHER: Time.lt ((View.rlx (TView.cur tview)) loc) to>>) /\
+    ((<<ORDW: Ordering.le ordw Ordering.strong_relaxed>>) \/
+     (<<ORDR: Ordering.le ord Ordering.strong_relaxed>>)).
+
+  Definition ww_race (loc: Loc.t) (to: Time.t) (ordw: Ordering.t) (tview: TView.t) (ord: Ordering.t): Prop :=
+    (<<LOC: L loc>>) /\
+    (<<HIGHER: Time.lt ((View.rlx (TView.cur tview)) loc) to>>) /\
+    ((<<ORDW1: Ordering.le ordw Ordering.na>>) \/
+     (<<ORDW2: Ordering.le ord Ordering.na>>)).
+
+  Definition ra_race (loc: Loc.t) (to: Time.t) (ordw: Ordering.t) (tview: TView.t) (e: ProgramEvent.t): Prop :=
+    (exists val ord,
+        (<<READ: ProgramEvent.is_reading e = Some (loc, val, ord)>>) /\
+        (<<WRRACE: wr_race loc to ordw tview ord>>)) \/
+    (exists val ord,
+        (<<WRITE: ProgramEvent.is_writing e = Some (loc, val, ord)>>) /\
+        (<<WWRACE: ww_race loc to ordw tview ord>>)).
+
+  Definition race (c1: Configuration.t): Prop :=
+    exists c2 c3
+      tid_w e_w loc from to val released ordw
+      tid_r lang st3 lc3 e st4,
+      (<<WRITE_STEP: OrdConfiguration.estep L Ordering.acqrel Ordering.acqrel e_w tid_w c1 c2>>) /\
+      (<<WRITE_EVENT: ThreadEvent.is_writing e_w = Some (loc, from, to, val, released, ordw)>>) /\
+      (<<STEPS2: rtc (@OrdConfiguration.all_step L Ordering.acqrel Ordering.acqrel) c2 c3>>) /\
+      (<<FIND: IdentMap.find tid_r (Configuration.threads c3) = Some (existT _ lang st3, lc3)>>) /\
+      (<<STEP: lang.(Language.step) e st3 st4>>) /\
+      (<<RACE: ra_race loc to ordw (Local.tview lc3) e>>).
+
+  Definition racefree (c: Configuration.t): Prop :=
+    forall c1 (STEPS1: rtc (@OrdConfiguration.all_step L Ordering.acqrel Ordering.acqrel) c c1),
+      ~ race c1.
+
+  Definition racefree_syn (s: Threads.syntax): Prop :=
+    racefree (Configuration.init s).
+
+
+  (* Lemma read_message_exists *)
+  (*       lang *)
+  (*       rels1 rels2 e1 e2 *)
+  (*       loc to ordw *)
+  (*       (LC_WF1: Local.wf (Thread.local e1) (Thread.global e1)) *)
+  (*       (GL_WF1: Global.wf (Thread.global e1)) *)
+  (*       (STEPS: @WThread.steps lang L Ordering.acqrel Ordering.acqrel rels1 rels2 e1 e2) *)
+  (*       (RELS2: List.In (loc, to, ordw) rels2) *)
+  (*       (HIGHER: Time.lt ((Local.tview (Thread.local e2)).(TView.cur).(View.rlx) loc) to): *)
+  (*   (<<RELS1: List.In (loc, to, ordw) rels1>>). *)
+  (* Proof. *)
+  (*   dependent induction STEPS; try by (esplits; eauto). *)
+  (*   hexploit WThread.step_reserve_only; try exact STEP; eauto. i. des. *)
+  (*   exploit WThread.step_future; eauto. i. des. *)
+  (*   exploit WThread.steps_future; try exact STEPS; eauto. i. des. *)
+  (*   exploit IHSTEPS; eauto. intros x. des. *)
+  (*   clear IHSTEPS. revert x. *)
+  (*   inv STEP. inv STEP0; inv STEP; [|inv LOCAL]; ss; try by (esplits; eauto). *)
+  (*   - unfold Writes.append. ss. condtac; ss. i. des; ss. inv x. *)
+  (*     assert (Time.le to ((TView.cur (Local.tview lc2)).(View.rlx) loc)). *)
+  (*     { inv LOCAL0. inv STEP. ss. *)
+  (*       unfold TimeMap.join, TimeMap.singleton. *)
+  (*       unfold LocFun.add, LocFun.init, LocFun.find. condtac; ss. *)
+  (*       apply Time.join_r. *)
+  (*     } *)
+  (*     inv TVIEW_FUTURE0. inv CUR. rewrite (RLX loc) in H0. timetac. *)
+  (*   - unfold Writes.append. ss. condtac; ss. i. des; ss. inv x. *)
+  (*     assert (Time.le to ((TView.cur (Local.tview lc2)).(View.rlx) loc)). *)
+  (*     { inv LOCAL2. inv STEP. ss. *)
+  (*       unfold TimeMap.join, TimeMap.singleton. *)
+  (*       unfold LocFun.add, LocFun.init, LocFun.find. condtac; ss. *)
+  (*       apply Time.join_r. *)
+  (*     } *)
+  (*     inv TVIEW_FUTURE0. inv CUR. rewrite (RLX loc) in H0. timetac. *)
+  (*   - unfold Writes.append. ss. condtac; ss. i. des; ss. inv x. *)
+  (*     assert (Time.le to ((TView.cur (Local.tview lc2)).(View.rlx) loc)). *)
+  (*     { inv LOCAL0. *)
+  (*       - inv STEP. ss. *)
+  (*         unfold TimeMap.join, TimeMap.singleton. *)
+  (*         unfold LocFun.add, LocFun.init, LocFun.find. condtac; ss. *)
+  (*         apply Time.join_r. *)
+  (*       - inv STEP. ss. *)
+  (*         unfold TimeMap.join, TimeMap.singleton. *)
+  (*         unfold LocFun.add, LocFun.init, LocFun.find. condtac; ss. *)
+  (*         apply Time.join_r. *)
+  (*     } *)
+  (*     inv TVIEW_FUTURE0. inv CUR. rewrite (RLX loc) in H0. timetac. *)
+  (* Qed. *)
+
+  Lemma write_exists
+        ordr ordw
+        rels1 rels2 c1 c2
+        loc to ord
+        (WF1: Configuration.wf c1)
+        (STEPS: WConfiguration.steps L ordr ordw rels1 rels2 c1 c2)
+        (LOC: L loc)
+        (RELS1: ~ List.In (loc, to, ord) rels1)
+        (RELS2: List.In (loc, to, ord) rels2):
+    exists rels11 rels12 c11 c12 tid e from val released,
+      (<<STEPS1: WConfiguration.steps L ordr ordw rels1 rels11 c1 c11>>) /\
+      (<<WRITE_STEP: WConfiguration.step L ordr ordw e tid rels11 rels12 c11 c12>>) /\
+      (<<WRITE_EVENT: ThreadEvent.is_writing e = Some (loc, from, to, val, released, ord)>>) /\
+      (<<STEPS2: WConfiguration.steps L ordr ordw rels12 rels2 c12 c2>>).
+  Proof.
+    revert WF1. induction STEPS; i; try congr.
+    exploit WConfiguration.step_future; eauto. i. des.
+    exploit WConfiguration.step_rels; eauto. i. subst.
+    destruct (classic (exists from val released,
+                          ThreadEvent.is_writing e = Some (loc, from, to, val, released, ord))).
+    { des. esplits; eauto. econs 1. }
+    exploit IHSTEPS; eauto.
+    { unfold Writes.append. des_ifs. ii. ss. des; ss. inv H0. eauto. }
+    i. des. esplits; eauto. econs 2; eauto.
+  Qed.
+
+  Lemma racefree_implies
+        s
+        (RACEFREE: racefree_syn s):
+    RARaceW.racefree_syn L Ordering.acqrel Ordering.acqrel s.
+  Proof.
+    specialize (@Configuration.init_wf s). intro WF.
+    ii. unfold RARaceW.ra_race in *. des.
+    { destruct WRRACE as [to [ordw [LOC [HIGHER [IN ORD]]]]]. guardH ORD. des.
+      unfold racefree_syn in *.
+      remember (Configuration.init s) as c1. clear Heqc1.
+      exploit write_exists; try exact STEPS; eauto. i. des.
+      exploit WConfiguration.steps_ord_steps; try exact STEPS1. i.
+      exploit WConfiguration.step_ord_step; try exact WRITE_STEP. i.
+      exploit WConfiguration.steps_ord_steps; try exact STEPS2. i.
+      eapply RACEFREE; eauto.
+      unfold race. esplits; eauto.
+      left. esplits; eauto.
+      unfold wr_race. splits; auto.
+    }
+    { destruct WWRACE as [to [ordw [LOC [HIGHER [IN ORD]]]]]. guardH ORD. des.
+      unfold racefree_syn in *.
+      remember (Configuration.init s) as c1. clear Heqc1.
+      exploit write_exists; try exact STEPS; eauto. i. des.
+      exploit WConfiguration.steps_ord_steps; try exact STEPS1. i.
+      exploit WConfiguration.step_ord_step; try exact WRITE_STEP. i.
+      exploit WConfiguration.steps_ord_steps; try exact STEPS2. i.
+      eapply RACEFREE; eauto.
+      unfold race. esplits; eauto.
+      right. esplits; eauto.
+      unfold ww_race. splits; auto.
+    }
+  Qed.
+End RARACE.
+End RARace.
